handle lists, pairs, and trepeat to get halve_spec automated

theories/Automation.v
@@ -1,10 +1,10 @@
+Require Import Coq.Lists.List Coq.Sorting.Permutation.
 
 From Coq Require Import ZArith.
 From ITree Require Export ITree.
 From Paco Require Import paco.
-Require Export Refinement.
-Require Import Merge.
-Require Import MergePartial.
+Require Import Lia.
+Require Export Refinement Merge MergePartial.
 
 Import Monads.
 Import MonadNotation.
@@ -77,6 +77,38 @@ Lemma padded_refines_if_l E1 E2 RE REAns R1 R2 RR (t1 t2 : itree_spec E1 R1) (t3
   padded_refines RE REAns RR (if b then t1 else t2) t3.
 Proof.
   intros. destruct b; eauto.
+Qed.
+
+Lemma padded_refines_match_list_r E1 E2 RE REAns R1 R2 RR A (t1 : itree_spec E1 R1)
+      (t2 : A -> list A -> itree_spec E2 R2) (t3 : itree_spec E2 R2) xs :
+  (forall x xs', xs = x :: xs' -> padded_refines RE REAns RR t1 (t2 x xs')) ->
+  (xs = nil -> padded_refines RE REAns RR t1 t3) ->
+  padded_refines RE REAns RR t1 (match xs with | x :: xs' => t2 x xs' | nil => t3 end).
+Proof.
+  intros. destruct xs; eauto.
+Qed.
+Lemma padded_refines_match_list_l E1 E2 RE REAns R1 R2 RR A (t3 : itree_spec E2 R2)
+      (t1 : A -> list A -> itree_spec E1 R1) (t2 : itree_spec E1 R1) xs :
+  (forall x xs', xs = x :: xs' -> padded_refines RE REAns RR (t1 x xs') t3) ->
+  (xs = nil -> padded_refines RE REAns RR t2 t3) ->
+  padded_refines RE REAns RR (match xs with | x :: xs' => t1 x xs' | nil => t2 end) t3.
+Proof.
+  intros. destruct xs; eauto.
+Qed.
+
+Lemma padded_refines_match_pair_r E1 E2 RE REAns R1 R2 RR A B
+      (t1 : itree_spec E1 R1) (t2 : A -> B -> itree_spec E2 R2) pr :
+  (forall x y, pr = (x, y) -> padded_refines RE REAns RR t1 (t2 x y)) ->
+  padded_refines RE REAns RR t1 (match pr with | (x,y) => t2 x y end).
+Proof.
+  intros. destruct pr; eauto.
+Qed.
+Lemma padded_refines_match_pair_l E1 E2 RE REAns R1 R2 RR A B
+      (t1 : A -> B -> itree_spec E1 R1) (t2 : itree_spec E2 R2) pr :
+  (forall x y, pr = (x, y) -> padded_refines RE REAns RR (t1 x y) t2) ->
+  padded_refines RE REAns RR (match pr with | (x,y) => t1 x y end) t2.
+Proof.
+  intros. destruct pr; eauto.
 Qed.
 
 Lemma padded_refines_ret_bind_r E1 E2 R1 R2 A
@@ -152,14 +184,14 @@ Context (E1 E2 : Type -> Type) (A1 A2 R1 R2 : Type).
 Context (RE : relationEH E1 E2) (REAns : relationEAns E1 E2) (RR : R1 -> R2 -> Prop).
 
 Context (precond : A1 -> A2 -> Prop)
-        (postcond : A1 -> A2 -> forall r1 r2, RR r1 r2 -> Prop).
+        (postcond : forall a1 a2, precond a1 a2 -> forall r1 r2, RR r1 r2 -> Prop).
 
 Variant padded_refines_rec_REInv : relationEH (callE A1 R1) (callE A2 R2) :=
   | padded_refines_rec_REInv_i a1 a2 : precond a1 a2 ->
     padded_refines_rec_REInv R1 R2 (Call a1) (Call a2).
 
 Variant padded_refines_rec_REAnsInv : relationEAns (callE A1 R1) (callE A2 R2) :=
-  | padded_refines_rec_REAnsInv_i a1 a2 r1 r2 : dep_prod_rel RR (postcond a1 a2) r1 r2 ->
+  | padded_refines_rec_REAnsInv_i a1 a2 r1 r2 p : dep_prod_rel RR (postcond a1 a2 p) r1 r2 ->
     padded_refines_rec_REAnsInv R1 R2 (Call a1) (Call a2) r1 r2.
 
 Context (body1 : A1 -> itree_spec (callE A1 R1 +' E1) R1)
@@ -167,10 +199,10 @@ Context (body1 : A1 -> itree_spec (callE A1 R1 +' E1) R1)
 
 Lemma padded_refines_rec_lr (a1 : A1) (a2 : A2) :
   precond a1 a2 ->
-  (forall a1 a2, precond a1 a2 ->
+  (forall a1 a2 (p : precond a1 a2),
      padded_refines (sum_relE padded_refines_rec_REInv RE)
                     (sum_relEAns padded_refines_rec_REAnsInv REAns)
-                    (dep_prod_rel RR (postcond a1 a2))
+                    (dep_prod_rel RR (postcond a1 a2 p))
                     (body1 a1) (body2 a2)) ->
   padded_refines RE REAns RR (mrec_spec (calling' body1) (Call a1))
                              (mrec_spec (calling' body2) (Call a2)).
@@ -182,12 +214,36 @@ Proof.
   eapply padded_refines_mrec with (REInv := padded_refines_rec_REInv)
                                   (REAnsInv := padded_refines_rec_REAnsInv).
   - intros A B [] [] []. unfold calling'.
-    eapply padded_refines_monot with (RR1 := dep_prod_rel RR (postcond a3 a4)); eauto.
-    intros. constructor; eauto.
+    eapply padded_refines_monot with (RR1 := dep_prod_rel RR (postcond a3 a4 H1)); eauto.
+    intros. econstructor; eauto.
   - constructor; eauto.
 Qed.
 
 End Rec.
+
+Lemma padded_refines_trepeat_zero_r E1 E2 R1 R2 RE REAns RR
+      (t1 : itree_spec E1 R1) (t2 : itree_spec E2 R2) :
+  padded_refines RE REAns RR t1 (Ret tt) ->
+  padded_refines RE REAns RR t1 (trepeat 0 t2).
+Proof. eauto. Qed.
+
+Lemma padded_refines_trepeat_suc_r E1 E2 R1 R2 RE REAns RR
+      (t1 : itree_spec E1 R1) n (t2 : itree_spec E2 R2) :
+  padded_refines RE REAns RR t1 (t2 ;; trepeat n t2) ->
+  padded_refines RE REAns RR t1 (trepeat (S n) t2).
+Proof. eauto. Qed.
+
+Lemma padded_refines_trepeat_bind_zero_r E1 E2 R1 R2 R3 RE REAns RR
+      (t1 : itree_spec E1 R1) (t2 : itree_spec E2 R2) (t3 : unit -> itree_spec E2 R3) :
+  padded_refines RE REAns RR t1 (t3 tt) ->
+  padded_refines RE REAns RR t1 (trepeat 0 t2 >>= t3).
+Proof. eauto. Qed.
+
+Lemma padded_refines_trepeat_bind_suc_r E1 E2 R1 R2 R3 RE REAns RR
+      (t1 : itree_spec E1 R1) n (t2 : itree_spec E2 R2) (t3 : unit -> itree_spec E2 R3) :
+  padded_refines RE REAns RR t1 (t2 ;; (trepeat n t2 >>= t3)) ->
+  padded_refines RE REAns RR t1 (trepeat (S n) t2 >>= t3).
+Proof. simpl; rewrite bind_bind; eauto. Qed.
 
 
 (** * Hint Database Definitions *)
@@ -197,20 +253,25 @@ Create HintDb prepostcond.
 
 Hint Extern 999 (padded_refines _ _ _ _ _) => shelve : refines.
 
-Definition Halt (goal : Type) := goal.
 Definition RelGoal (goal : Prop) := goal.
 
-Hint Opaque Halt : refines.
 Hint Opaque RelGoal : refines.
 
-Hint Extern 999 (Halt _) => unfold Halt; shelve : refines.
 Hint Extern 999 (RelGoal _) =>
   unfold RelGoal; (reflexivity || shelve) : refines.
+
+Lemma padded_refines_eq_unfold E R1 R2 RR (t1 : itree_spec E R1) (t2 : itree_spec E R2) :
+  padded_refines eqE eqEAns RR t1 t2 ->
+  padded_refines_eq RR t1 t2.
+Proof. eauto. Qed.
+
+Hint Extern 100 (padded_refines_eq _ _ _) =>
+  simple apply padded_refines_eq_unfold : refines.
 
 
 (** * IntroArg Definition and Hints *)
 
-Inductive ArgName := Any | RetAny | Hyp | Exists | Forall | If.
+Inductive ArgName := Any | RetAny | Hyp | Exists | Forall | If | Match.
 Ltac argName n :=
   match n with
   | Any      => fresh "a"
@@ -219,56 +280,72 @@ Ltac argName n :=
   | Exists   => fresh "e_exists"
   | Forall   => fresh "e_forall"
   | If       => fresh "e_if"
+  | Match    => fresh "e_match"
   end.
 
-Definition IntroArg (n : ArgName) A (goal : A -> Type) := forall a, goal a.
+Polymorphic Definition IntroArg (n : ArgName) A (goal : A -> Type) := forall a, goal a.
 
 Hint Opaque IntroArg : refines prepostcond.
 
-Lemma IntroArg_fold n A goal : forall a, IntroArg n A goal -> goal a.
+Polymorphic Lemma IntroArg_fold n A goal : forall a, IntroArg n A goal -> goal a.
 Proof. intros a H; exact (H a). Qed.
 
-(* Lemma IntroArg_unfold n A (goal : A -> Prop) : (forall a, goal a) -> IntroArg n A goal. *)
+(* Polymorphic Lemma IntroArg_unfold n A (goal : A -> Prop) : (forall a, goal a) -> IntroArg n A goal. *)
 (* Proof. unfold IntroArg; intro H; exact H. Qed. *)
 
 Ltac IntroArg_intro e := intro e.
 
 Ltac IntroArg_forget := let e := fresh in intro e; clear e.
 
-Lemma IntroArg_sum_relE_inl n E1 E2 F1 F2 (REE : relationEH E1 E2) (REF : relationEH F1 F2)
-                            A B e1 e2 (goal : _ -> Prop) :
+Polymorphic Lemma IntroArg_eta n A (f : A -> Type) x goal :
+  IntroArg n (f x) goal ->
+  IntroArg n ((fun x' => f x') x) goal.
+Proof. eauto. Qed.
+
+Polymorphic Lemma IntroArg_and n P Q (goal : P /\ Q -> Prop)
+  : IntroArg n P (fun p => IntroArg n Q (fun q => goal (conj p q))) -> IntroArg n _ goal.
+Proof. intros H [ p q ]; apply H. Qed.
+
+Polymorphic Lemma IntroArg_sum_relE_inl n E1 E2 F1 F2
+                  (REE : relationEH E1 E2) (REF : relationEH F1 F2)
+                  A B e1 e2 (goal : _ -> Prop) :
   IntroArg n (REE A B e1 e2) (fun p => goal (sum_relE_inl _ _ _ _ _ _ p)) ->
   IntroArg n (@sum_relE E1 E2 F1 F2 REE REF A B (inl1 e1) (inl1 e2)) goal.
 Proof. intros ?H ?H; dependent destruction H0; apply H. Qed.
-Lemma IntroArg_sum_relE_inr n E1 E2 F1 F2 (REE : relationEH E1 E2) (REF : relationEH F1 F2)
-                            A B f1 f2 (goal : _ -> Prop) :
+Polymorphic Lemma IntroArg_sum_relE_inr n E1 E2 F1 F2
+                  (REE : relationEH E1 E2) (REF : relationEH F1 F2)
+                  A B f1 f2 (goal : _ -> Prop) :
   IntroArg n (REF A B f1 f2) (fun p => goal (sum_relE_inr _ _ _ _ _ _ p)) ->
   IntroArg n (@sum_relE E1 E2 F1 F2 REE REF A B (inr1 f1) (inr1 f2)) goal.
 Proof. intros ?H ?H; dependent destruction H0; apply H. Qed.
 
-Lemma IntroArg_sum_relEAns_inl n E1 E2 F1 F2 (REE : relationEAns E1 E2) (REF : relationEAns F1 F2)
-                               A B e1 e2 a b (goal : _ -> Prop) :
+Polymorphic Lemma IntroArg_sum_relEAns_inl n E1 E2 F1 F2
+                  (REE : relationEAns E1 E2) (REF : relationEAns F1 F2)
+                  A B e1 e2 a b (goal : _ -> Prop) :
   IntroArg n (REE A B e1 e2 a b) (fun p => goal (sum_relEAns_inl _ _ _ _ _ _ _ _ p)) ->
   IntroArg n (@sum_relEAns E1 E2 F1 F2 REE REF A B (inl1 e1) (inl1 e2) a b) goal.
 Proof. intros ?H ?H; dependent destruction H0; apply H. Qed.
-Lemma IntroArg_sum_relEAns_inr n E1 E2 F1 F2 (REE : relationEAns E1 E2) (REF : relationEAns F1 F2)
-                               A B f1 f2 a b (goal : _ -> Prop) :
+Polymorphic Lemma IntroArg_sum_relEAns_inr n E1 E2 F1 F2
+                  (REE : relationEAns E1 E2) (REF : relationEAns F1 F2)
+                  A B f1 f2 a b (goal : _ -> Prop) :
   IntroArg n (REF A B f1 f2 a b) (fun p => goal (sum_relEAns_inr _ _ _ _ _ _ _ _ p)) ->
   IntroArg n (@sum_relEAns E1 E2 F1 F2 REE REF A B (inr1 f1) (inr1 f2) a b) goal.
 Proof. intros ?H ?H; dependent destruction H0; apply H. Qed.
 
-Lemma IntroArg_padded_refines_rec_REInv_i n A1 A2 R1 R2 (precond : A1 -> A2 -> Prop)
-                                          a1 a2 (goal : _ -> Prop) :
+Polymorphic Lemma IntroArg_padded_refines_rec_REInv_i n A1 A2 R1 R2
+                  (precond : A1 -> A2 -> Prop) a1 a2 (goal : _ -> Prop) :
   IntroArg n (precond a1 a2) (fun p => goal (padded_refines_rec_REInv_i _ _ _ _ _ _ _ p)) ->
   IntroArg n (padded_refines_rec_REInv A1 A2 R1 R2 precond R1 R2 (Call a1) (Call a2)) goal.
 Proof. intros ?H ?H; dependent destruction H0; apply H. Qed.
 
-Lemma IntroArg_padded_refines_rec_REAnsInv_i n A1 A2 R1 R2 (RR : R1 -> R2 -> Prop)
-                                             (postcond : A1 -> A2 -> forall (r1 : R1) (r2 : R2), RR r1 r2 -> Prop)
-                                             a1 a2 r1 r2 (goal : _ -> Prop) :
-  IntroArg n (RR r1 r2) (fun p1 => IntroArg n (postcond a1 a2 r1 r2 p1) (fun p2 =>
-    goal (padded_refines_rec_REAnsInv_i _ _ _ _ _ _ _ _ _ _ (exist _ p1 p2)))) ->
-  IntroArg n (padded_refines_rec_REAnsInv A1 A2 R1 R2 RR postcond R1 R2 (Call a1) (Call a2) r1 r2) goal.
+Polymorphic Lemma IntroArg_padded_refines_rec_REAnsInv_i n A1 A2 R1 R2
+                  (RR : R1 -> R2 -> Prop) (precond : A1 -> A2 -> Prop)
+                  (postcond : forall a1 a2, precond a1 a2 -> forall (r1 : R1) (r2 : R2), RR r1 r2 -> Prop)
+                  a1 a2 r1 r2 (goal : _ -> Prop) :
+  IntroArg n (precond a1 a2) (fun p0 => IntroArg n (RR r1 r2) (fun p1 =>
+  IntroArg n (postcond a1 a2 p0 r1 r2 p1) (fun p2 =>
+    goal (padded_refines_rec_REAnsInv_i _ _ _ _ _ _ _ _ _ _ _ p0 (exist _ p1 p2))))) ->
+  IntroArg n (padded_refines_rec_REAnsInv A1 A2 R1 R2 RR precond postcond R1 R2 (Call a1) (Call a2) r1 r2) goal.
 Proof. intros ?H ?H; dependent destruction H0; dependent destruction d; apply H. Qed.
 
 Ltac IntroArg_intro_dependent_destruction n :=
@@ -279,6 +356,8 @@ Check dep_prod_rel.
 
 Ltac IntroArg_base_tac n A g :=
   lazymatch A with
+  | (fun _ => _) _ => simple apply IntroArg_eta
+  | _ /\ _ => simple apply IntroArg_and
   | sum_relE _ _ _ _ (inl1 _) (inl1 _) => simple apply IntroArg_sum_relE_inl
   | sum_relE _ _ _ _ (inr1 _) (inr1 _) => simple apply IntroArg_sum_relE_inr
   | sum_relE _ _ _ _ (inl1 _) (inr1 _) => IntroArg_intro_dependent_destruction n
@@ -288,7 +367,7 @@ Ltac IntroArg_base_tac n A g :=
   | sum_relEAns _ _ _ _ (inl1 _) (inr1 _) _ _ => IntroArg_intro_dependent_destruction n
   | sum_relEAns _ _ _ _ (inr1 _) (inl1 _) _ _ => IntroArg_intro_dependent_destruction n
   | padded_refines_rec_REInv _ _ _ _ _ _ _ (Call _) (Call _) => simple apply IntroArg_padded_refines_rec_REInv_i
-  | padded_refines_rec_REAnsInv _ _ _ _ _ _ _ _ (Call _) (Call _) _ _ => simple apply IntroArg_padded_refines_rec_REAnsInv_i
+  | padded_refines_rec_REAnsInv _ _ _ _ _ _ _ _ _ (Call _) (Call _) _ _ => simple apply IntroArg_padded_refines_rec_REAnsInv_i
   | true  = true  => IntroArg_intro_dependent_destruction n
   | false = false => IntroArg_intro_dependent_destruction n
   | true  = false => IntroArg_intro_dependent_destruction n
@@ -299,7 +378,7 @@ Hint Extern 101 (IntroArg ?n ?A ?g) => IntroArg_base_tac n A g : refines prepost
 
 Ltac IntroArg_rewrite_bool_eq n :=
   let e := fresh in
-    IntroArg_intro e; repeat rewrite e in *;
+    IntroArg_intro e; progress (repeat rewrite e in *);
     apply (IntroArg_fold n _ _ e); clear e.
 
 Hint Extern 102 (IntroArg ?n (@eq bool _ _) _) =>
@@ -307,12 +386,19 @@ Hint Extern 102 (IntroArg ?n (@eq bool _ _) _) =>
 
 Hint Extern 105 (IntroArg ?n (?x = ?y) _) =>
   let e := argName n in IntroArg_intro e;
-    try first [ is_var x; subst x | is_var y; subst y ] : refinesprepostcond .
+    try first [ is_var x; subst x | is_var y; subst y ] : refines.
 Hint Extern 106 (IntroArg ?n _ _) =>
   let e := argName n in IntroArg_intro e : refines prepostcond.
 
 
 (** * Hints for Relation Goals *)
+
+Lemma RelGoal_eta A (f : A -> Prop) x :
+  RelGoal (f x) -> RelGoal ((fun x' => f x') x).
+Proof. eauto. Qed.
+
+Hint Extern 101 (RelGoal ((fun _ => _) _)) =>
+  simple apply RelGoal_eta.
 
 Lemma RelGoal_sum_relE_inl E1 E2 F1 F2 (REE : relationEH E1 E2) (REF : relationEH F1 F2)
                            A B e1 e2 :
@@ -346,8 +432,8 @@ Hint Extern 101 (RelGoal (sum_relEAns _ _ _ _ (inl1 _) (inl1 _) _ _)) =>
 Hint Extern 101 (RelGoal (sum_relEAns _ _ _ _ (inr1 _) (inr1 _) _ _)) =>
   simple apply RelGoal_sum_relEAns_inr : refines.
 
-Lemma RelGoal_padded_refines_rec_REInv_i A1 A2 R1 R2 (precond : A1 -> A2 -> Prop)
-                                         a1 a2 :
+Lemma RelGoal_padded_refines_rec_REInv_i A1 A2 R1 R2
+      (precond : A1 -> A2 -> Prop)  a1 a2 :
   RelGoal (precond a1 a2) ->
   RelGoal (padded_refines_rec_REInv A1 A2 R1 R2 precond R1 R2 (Call a1) (Call a2)).
 Proof. constructor; eauto. Qed.
@@ -355,14 +441,15 @@ Proof. constructor; eauto. Qed.
 Hint Extern 101 (RelGoal (padded_refines_rec_REInv _ _ _ _ _ _ _ (Call _) (Call _))) =>
   simple apply RelGoal_padded_refines_rec_REInv_i : refines.
 
-Lemma RelGoal_padded_refines_rec_REAnsInv_i A1 A2 R1 R2 (RR : R1 -> R2 -> Prop)
-                                            (postcond : A1 -> A2 -> forall (r1 : R1) (r2 : R2), RR r1 r2 -> Prop)
-                                            a1 a2 r1 r2 :
-  forall (p1 : RelGoal (RR r1 r2)), RelGoal (postcond a1 a2 r1 r2 p1) ->
-  RelGoal (padded_refines_rec_REAnsInv A1 A2 R1 R2 RR postcond R1 R2 (Call a1) (Call a2) r1 r2).
-Proof. constructor; econstructor; eauto. Qed.
+Lemma RelGoal_padded_refines_rec_REAnsInv_i A1 A2 R1 R2
+      (RR : R1 -> R2 -> Prop) (precond : A1 -> A2 -> Prop)
+      (postcond : forall a1 a2, precond a1 a2 -> forall (r1 : R1) (r2 : R2), RR r1 r2 -> Prop)
+      a1 a2 r1 r2 :
+  forall (p0 : precond a1 a2) (p1 : RelGoal (RR r1 r2)), RelGoal (postcond a1 a2 p0 r1 r2 p1) ->
+  RelGoal (padded_refines_rec_REAnsInv A1 A2 R1 R2 RR precond postcond R1 R2 (Call a1) (Call a2) r1 r2).
+Proof. econstructor; econstructor; eauto. Qed.
 
-Hint Extern 101 (RelGoal (padded_refines_rec_REAnsInv _ _ _ _ _ _ _ _ (Call _) (Call _) _ _)) =>
+Hint Extern 101 (RelGoal (padded_refines_rec_REAnsInv _ _ _ _ _ _ _ _ _ (Call _) (Call _) _ _)) =>
   simple apply RelGoal_padded_refines_rec_REAnsInv_i : refines.
 
 Lemma RelGoal_dep_prod_rel {R1 R2} (RR1 : R1 -> R2 -> Prop) (RR2 : forall r1 r2, RR1 r1 r2 -> Prop) r1 r2 :
@@ -414,23 +501,23 @@ Definition padded_spec_forall_r_IntroArg E1 E2 R1 R2 A
   padded_refines RE REAns RR phi (Vis Spec_forall kphi) :=
   padded_spec_forall_r E1 E2 R1 R2 A RE REAns RR phi kphi.
 
-Hint Extern 102 (padded_refines _ _ _ (Vis Spec_forall _)) =>
-  simple apply padded_spec_forall_l : refines.
-Hint Extern 102 (padded_refines _ _ _ (vis Spec_forall _)) =>
-  apply padded_spec_forall_l : refines.
-Hint Extern 102 (padded_refines _ _ _ _ (Vis Spec_exists _)) =>
-  simple apply padded_spec_exists_r : refines.
-Hint Extern 102 (padded_refines _ _ _ _ (vis Spec_exists _)) =>
-  apply padded_spec_exists_r : refines.
+Hint Extern 102 (padded_refines _ _ _ _ (Vis Spec_forall _)) =>
+  unshelve (simple apply padded_spec_forall_r); [shelve|] : refines.
+Hint Extern 102 (padded_refines _ _ _ _ (vis Spec_forall _)) =>
+  unshelve (apply padded_spec_forall_r); [shelve|] : refines.
+Hint Extern 102 (padded_refines _ _ _ (Vis Spec_exists _) _) =>
+  unshelve (simple apply padded_spec_exists_l); [shelve|] : refines.
+Hint Extern 102 (padded_refines _ _ _ (vis Spec_exists _) _) =>
+  unshelve (apply padded_spec_exists_l); [shelve|] : refines.
 
 Hint Extern 103 (padded_refines _ _ _ _ (Vis Spec_exists _)) =>
-  simple eapply padded_spec_exists_r : refines.
+  unshelve (simple eapply padded_spec_exists_r); [shelve|] : refines.
 Hint Extern 103 (padded_refines _ _ _ _ (vis Spec_exists _)) =>
-  eapply padded_spec_exists_r : refines.
+  unshelve (eapply padded_spec_exists_r); [shelve|] : refines.
 Hint Extern 103 (padded_refines _ _ _ (Vis Spec_forall _) _) =>
-  simple eapply padded_spec_forall_l : refines.
+  unshelve (simple eapply padded_spec_forall_l); [shelve|] : refines.
 Hint Extern 103 (padded_refines _ _ _ (vis Spec_forall _) _) =>
-  eapply padded_spec_forall_l : refines.
+  unshelve (eapply padded_spec_forall_l); [shelve|] : refines.
 
 Definition padded_refines_if_r_IntroArg E1 E2 RE REAns R1 R2 RR t1 t2 t3 b :
   (IntroArg If (b = true) (fun _ => padded_refines RE REAns RR t1 t2)) ->
@@ -447,6 +534,44 @@ Hint Extern 101 (padded_refines _ _ _ _ (if _ then _ else _)) =>
   apply padded_refines_if_r_IntroArg : refines.
 Hint Extern 101 (padded_refines _ _ _ (if _ then _ else _) _) =>
   apply padded_refines_if_l_IntroArg : refines.
+
+Definition padded_refines_match_list_r_IntroArg E1 E2 RE REAns R1 R2 RR A (t1 : itree_spec E1 R1)
+      (t2 : A -> list A -> itree_spec E2 R2) (t3 : itree_spec E2 R2) xs :
+  (IntroArg Any A (fun x => IntroArg Any (list A) (fun xs' =>
+   IntroArg Match (xs = x :: xs') (fun _ => padded_refines RE REAns RR t1 (t2 x xs'))))) ->
+  (IntroArg Match (xs = nil) (fun _ => padded_refines RE REAns RR t1 t3)) ->
+  padded_refines RE REAns RR t1 (match xs with | x :: xs' => t2 x xs' | nil => t3 end) :=
+  padded_refines_match_list_r E1 E2 RE REAns R1 R2 RR A t1 t2 t3 xs.
+Definition padded_refines_match_list_l_IntroArg E1 E2 RE REAns R1 R2 RR A (t3 : itree_spec E2 R2)
+      (t1 : A -> list A -> itree_spec E1 R1) (t2 : itree_spec E1 R1) xs :
+  (IntroArg Any A (fun x => IntroArg Any (list A) (fun xs' =>
+   IntroArg Match (xs = x :: xs') (fun _ => padded_refines RE REAns RR (t1 x xs') t3)))) ->
+  (IntroArg Match (xs = nil) (fun _ => padded_refines RE REAns RR t2 t3)) ->
+  padded_refines RE REAns RR (match xs with | x :: xs' => t1 x xs' | nil => t2 end) t3 :=
+  padded_refines_match_list_l E1 E2 RE REAns R1 R2 RR A t3 t1 t2 xs.
+
+Hint Extern 101 (padded_refines _ _ _ _ (match _ with | _ :: _ => _ | nil => _ end)) =>
+  apply padded_refines_match_list_r_IntroArg : refines.
+Hint Extern 101 (padded_refines _ _ _ (match _ with | _ :: _ => _ | nil => _ end) _) =>
+  apply padded_refines_match_list_l_IntroArg : refines.
+
+Definition padded_refines_match_pair_r_IntroArg E1 E2 RE REAns R1 R2 RR A B
+      (t1 : itree_spec E1 R1) (t2 : A -> B -> itree_spec E2 R2) pr :
+  (IntroArg Any A (fun x => IntroArg Any B (fun y => 
+   IntroArg Match (pr = (x, y)) (fun _ => padded_refines RE REAns RR t1 (t2 x y))))) ->
+  padded_refines RE REAns RR t1 (match pr with | (x,y) => t2 x y end) :=
+  padded_refines_match_pair_r E1 E2 RE REAns R1 R2 RR A B t1 t2 pr.
+Definition padded_refines_match_pair_l_IntroArg E1 E2 RE REAns R1 R2 RR A B
+      (t1 : A -> B -> itree_spec E1 R1) (t2 : itree_spec E2 R2) pr :
+  (IntroArg Any A (fun x => IntroArg Any B (fun y => 
+   IntroArg Match (pr = (x, y)) (fun _ => padded_refines RE REAns RR (t1 x y) t2)))) ->
+  padded_refines RE REAns RR (match pr with | (x,y) => t1 x y end) t2 :=
+  padded_refines_match_pair_l E1 E2 RE REAns R1 R2 RR A B t1 t2 pr.
+
+Hint Extern 101 (padded_refines _ _ _ _ (match _ with | (_,_) => _ end)) =>
+  apply padded_refines_match_pair_r_IntroArg : refines.
+Hint Extern 101 (padded_refines _ _ _ (match _ with | (_,_) => _ end) _) =>
+  apply padded_refines_match_pair_l_IntroArg : refines.
 
 Hint Extern 101 (padded_refines _ _ _ _ (Ret _ >>= _)) =>
   simple apply padded_refines_ret_bind_r : refines.
@@ -530,33 +655,43 @@ Hint Extern 101 (padded_refines _ _ _ (spec_forall _ >>= _) _) =>
 (** * Refinement Hints About Recursion *)
 
 Definition Precondition {A1 A2} (a1 : A1) (a2 : A2) := Prop.
-Definition Postcondition {A1 A2 R1 R2 RR} (a1 : A1) (a2 : A2)
-                         (r1 : R1) (r2 : R2) (H : (RR r1 r2 : Prop)) := Prop.
+Definition Postcondition {A1 A2 R1 R2 precond RR} (a1 : A1) (a2 : A2) (H : precond a1 a2)
+                         (r1 : R1) (r2 : R2) (H0 : (RR r1 r2 : Prop)) := Prop.
+Definition Continue (precond : Prop) (goal : Type) := (precond * goal)%type.
 
 Hint Opaque Precondition : prepostcond.
 Hint Opaque Postcondition : prepostcond.
+Hint Opaque Continue : prepostcond.
+
+Lemma Continue_unfold precond goal :
+  RelGoal precond -> goal -> Continue precond goal.
+Proof. split; eauto. Qed.
 
 Hint Extern 999 (Precondition _ _) => shelve : prepostcond.
-Hint Extern 999 (Postcondition _ _ _ _ _) => shelve : prepostcond.
+Hint Extern 999 (Postcondition _ _ _ _ _ _) => shelve : prepostcond.
+Hint Extern 999 (Continue _ _) => shelve : refines.
 
 Definition padded_refines_rec_lr_IntroArg
            E1 E2 A1 A2 R1 R2 RE REAns (RR : R1 -> R2 -> Prop) body1 body2 a1 a2
            (precond : IntroArg Any A1 (fun a1 => IntroArg Any A2 (fun a2 => Precondition a1 a2)))
            (postcond : IntroArg Any A1 (fun a1 => IntroArg Any A2 (fun a2 =>
+                       IntroArg Hyp (precond a1 a2) (fun H =>
                        IntroArg RetAny R1 (fun r1 => IntroArg RetAny R2 (fun r2 =>
-                       IntroArg Hyp (RR r1 r2) (fun H => Postcondition a1 a2 r1 r2 H)))))) :
-  precond a1 a2 ->
-  (IntroArg Any A1 (fun a1 => IntroArg Any A2 (fun a2 =>
-   IntroArg Hyp (precond a1 a2) (fun _ => Halt (
-     padded_refines (sum_relE _ RE)
-                    (sum_relEAns _ REAns)
-                    (dep_prod_rel RR (postcond a1 a2))
-                    (body1 a1) (body2 a2)))))) ->
+                       IntroArg Hyp (RR r1 r2) (fun H0 => Postcondition a1 a2 H r1 r2 H0))))))) :
+  Continue (precond a1 a2)
+           (IntroArg Any A1 (fun a1 => IntroArg Any A2 (fun a2 =>
+            IntroArg Hyp (precond a1 a2) (fun p =>
+            padded_refines (sum_relE _ RE)
+                           (sum_relEAns _ REAns)
+                           (dep_prod_rel RR (postcond a1 a2 p))
+                           (body1 a1) (body2 a2))))) ->
   padded_refines RE REAns RR (mrec_spec (calling' body1) (Call a1))
-                 (mrec_spec (calling' body2) (Call a2)) :=
-  padded_refines_rec_lr E1 E2 A1 A2 R1 R2 RE REAns RR precond postcond body1 body2 a1 a2.
+                             (mrec_spec (calling' body2) (Call a2)) := fun pr =>
+  match pr with
+  | (p, q) => padded_refines_rec_lr E1 E2 A1 A2 R1 R2 RE REAns RR precond postcond body1 body2 a1 a2 p q
+  end.
 
-Ltac padded_refines_rec := eapply padded_refines_rec_lr_IntroArg; [shelve | idtac].
+Ltac padded_refines_rec := eapply padded_refines_rec_lr_IntroArg.
 
 Hint Extern 101 (padded_refines _ _ _ (mrec_spec (calling' _) (Call _))
                                       (mrec_spec (calling' _) (Call _))) =>
@@ -568,6 +703,24 @@ Hint Extern 101 (padded_refines _ _ _ (rec_fix_spec _ _) (rec_fix_spec _ _)) =>
 
 Hint Extern 101 (padded_refines _ _ _ (call_spec _) (call_spec _)) =>
   apply padded_refines_trigger_l, padded_refines_trigger_r : refines.
+Hint Extern 101 (padded_refines _ _ _ _ (call_spec _ >>= _)) =>
+  apply padded_refines_trigger_bind_r : refines.
+Hint Extern 101 (padded_refines _ _ _ (call_spec _ >>= _) _) =>
+  apply padded_refines_trigger_bind_l : refines.
+
+Hint Extern 991 (padded_refines _ _ _ (Vis (Spec_vis (inl1 (Call _) )) _) (trepeat _ _)) =>
+  simple apply padded_refines_trepeat_suc_r : refines.
+Hint Extern 991 (padded_refines _ _ _ (vis (Spec_vis (inl1 (Call _) )) _) (trepeat _ _)) =>
+  simple apply padded_refines_trepeat_suc_r : refines.
+Hint Extern 991 (padded_refines _ _ _ (Vis (Spec_vis (inl1 (Call _) )) _) (trepeat _ _ >>= _)) =>
+  simple apply padded_refines_trepeat_bind_suc_r : refines.
+Hint Extern 991 (padded_refines _ _ _ (vis (Spec_vis (inl1 (Call _) )) _) (trepeat _ _ >>= _)) =>
+  simple apply padded_refines_trepeat_bind_suc_r : refines.
+
+Hint Extern 992 (padded_refines _ _ _ _ (trepeat _ _)) =>
+  simple apply padded_refines_trepeat_zero_r : refines.
+Hint Extern 992 (padded_refines _ _ _ _ (trepeat _ _ >>= _)) =>
+  simple apply padded_refines_trepeat_bind_zero_r : refines.
 
 
 (** * Tactics *)
@@ -580,6 +733,9 @@ Ltac prove_refinement_prepostcond :=
 
 Ltac prove_refinement :=
   prove_refinement_eauto; prove_refinement_prepostcond.
+
+Ltac prove_refinement_continue :=
+  apply Continue_unfold; prove_refinement.
 
 
 (** * Examples *)
@@ -602,8 +758,7 @@ Proof.
   prove_refinement.
   - exact True.
   - exact True.
-  - easy.
-  - prove_refinement.
+  - prove_refinement_continue.
 Qed.
 
 Lemma test_exists E (x : Z) :
@@ -612,4 +767,35 @@ Lemma test_exists E (x : Z) :
                   (r <- spec_exists Z ;; Ret r).
 Proof.
   prove_refinement.
+Qed.
+
+Lemma test_halve_refl E xs :
+  padded_refines_eq eq (@halve E xs) (@halve E xs).
+Proof.
+  unfold padded_refines_eq, halve.
+  prove_refinement.
+  - exact (a = a0).
+  - exact True.
+  - prove_refinement_continue.
+Qed.
+
+Open Scope nat_scope.
+
+Lemma halve_refines_spec E l :
+  padded_refines_eq eq (@halve E l) (@halve_spec_fix E l).
+Proof.
+  unfold halve, halve_spec_fix, halve_spec.
+  prove_refinement.
+  - exact (a = a0).
+  - exact ((Permutation a (fst r ++ snd r)) /\
+           (length (fst r) >= length (snd r) /\ (length a > length (fst r) \/ length a <= 1))).
+  - prove_refinement_continue.
+    all: cbn; cbn in *.
+    all: try split; try easy; try lia.
+    + rewrite Permutation_app_comm. cbn.
+      rewrite H0. rewrite Permutation_app_comm. reflexivity.
+    + rewrite H0. repeat rewrite app_length. lia.
+    + rewrite Permutation_app_comm. cbn.
+      rewrite H0. rewrite Permutation_app_comm. reflexivity.
+    + repeat rewrite H0. repeat rewrite app_length. lia.
 Qed.
